extraction (WIP)

minuska/theories/basic_matching.v
@@ -1437,26 +1437,6 @@ Section with_signature.
 
 End with_signature.
 
-Class ComputableSignature {Σ : Signature} := {
-    builtin_unary_predicate_interp_bool :
-        builtin_unary_predicate -> GroundTerm -> bool ; 
-
-    builtin_binary_predicate_interp_bool :
-        builtin_binary_predicate -> GroundTerm -> GroundTerm -> bool ;         
-
-    cs_up :
-        forall p e,
-            reflect
-                (builtin_unary_predicate_interp p e)
-                (builtin_unary_predicate_interp_bool p e) ;
-
-    cs_bp :
-        forall p e1 e2,
-            reflect
-                (builtin_binary_predicate_interp p e1 e2)
-                (builtin_binary_predicate_interp_bool p e1 e2) ;
-}.
-
 Definition val_satisfies_ap_bool
     `{ComputableSignature}
     (ρ : Valuation)
