minuska/theories/examples.v
@@ -1,11 +1,14 @@
 From Coq.Logic Require Import ProofIrrelevance.
 
+Require Extraction.
+
 From Minuska Require Import
     prelude
     spec_syntax
     spec_semantics
     string_variables
     empty_builtin
+    flattened
     naive_interpreter
 .
 
@@ -26,6 +29,20 @@ Module example_1.
         apply EmptyBuiltin.
     Defined.
 
+
+    Program Instance CΣ : @ComputableSignature Σ := {|
+        builtin_unary_predicate_interp_bool := fun _ _ => false ;
+        builtin_binary_predicate_interp_bool := fun _ _ _ => false ;
+    |}.
+    Next Obligation.
+        destruct p.
+    Qed.
+    Next Obligation.
+        destruct p.
+    Qed.
+    Fail Next Obligation.
+
+    (*
     Definition left_SSX : LhsPattern :=
         (aoo_operand _ _
             (wsc_base
@@ -98,5 +115,44 @@ Module example_1.
         unfold left_SSX, right_X.
         repeat constructor.
     Qed.
+
+    *)
+
+    Print GroundTerm.
+    Print BuiltinOrVar.
+    Print OpenTerm.
+    Print AppliedOperatorOr'.
+    Print AppliedOperator'.
+    Print RhsPattern.
+    Print Expression.
+
+    Definition rule_1 : FlattenedRewritingRule := {|
+        fr_from := aoo_app _ _  (ao_app_ao (ao_operator "s") ((ao_app_operand (ao_operator "s") (bov_variable "X"))));
+        fr_to := aoo_operand _ _  (ft_variable "X");
+        fr_scs := [] ;
+    |}.
+
+    Definition Γ : FlattenedRewritingTheory := [rule_1].
+
+    Definition interp :=
+        naive_interpreter Γ
+    .
+
+    Fixpoint my_number' (n : nat) : AppliedOperator' symbol builtin_value  :=
+    match n with
+    | 0 => ao_operator "0"
+    | S n' => ao_app_ao (ao_operator "s") (my_number' n')
+    end
+    .
+
+    Definition my_number (n : nat) : GroundTerm :=
+        aoo_app _ _ (my_number' n)
+    .
+
+
+    Compute (my_number 2).
+    Compute (interp (my_number 2)).
+
+    Extraction "example_lang" interp.
 
 End example_1.
